MMU_ARMv7_Refinement_No_Fault/ARMv7_Address_Translate_Ref.thy
@@ -89,8 +89,6 @@ definition
 end
 
 
-(* should we use history or not, for translation *)
-
 
 instantiation tlb_incon_state'_ext :: (type) mmu    
 begin
@@ -111,6 +109,29 @@ definition
 
   instance ..
 end
+
+
+
+instantiation tlb_incon_state'2_ext :: (type) mmu    
+begin
+definition   
+ "(mmu_translate v :: ('a tlb_incon_state'2_scheme \<Rightarrow> _))
+  = do {
+     mem   <- read_state MEM;
+     asid  <- read_state ASID;
+     ttbr0 <- read_state TTBR0;
+     tlb_incon_set <- read_state tlb_incon_set'2;
+     if  v \<in> incon_set2 tlb_incon_set
+       then raise'exception (IMPLEMENTATION_DEFINED ''set on fire'')
+       else let entry = pt_walk asid mem ttbr0 v in 
+             if is_fault entry
+              then raise'exception (PAGE_FAULT ''more info'')
+              else return (Addr (va_to_pa (addr_val v) entry))
+    }"
+
+  instance ..
+end
+
 
 
 lemma lookup_miss_tlb_subset1:
@@ -541,5 +562,74 @@ lemma mmu_translate_sat_no_flt_abs_refine:
           (ASID t,  va) \<notin> incon_set(tlb_incon_set' t) ; tlb_rel_abs' (typ_sat_no_flt_tlb s) (typ_incon' t) \<rbrakk> \<Longrightarrow> 
                               pa = pa' \<and>  (ASID t',  va) \<notin> incon_set(tlb_incon_set' t') \<and> tlb_rel_abs'  (typ_sat_no_flt_tlb s') (typ_incon' t')"
   by (clarsimp simp: mmu_translate_sat_abs_refine_pa' mmu_translate_sat_abs_refine' mmu_translate_sat_abs_refine_consistency)
+
+
+
+
+(* refinement between two abstracted levels  *)
+
+
+
+lemma tlb_rel_abs_consistent'2 [simp]:
+  "\<lbrakk>va \<notin> incon_set2 (tlb_incon_set'2 t) ;   tlb_rel_abs'2 (typ_incon' s) (typ_incon'2 t) \<rbrakk>  \<Longrightarrow> 
+           (ASID s, va) \<notin> incon_set (tlb_incon_set' s) " 
+  apply (clarsimp simp: tlb_rel_abs'2_def)
+  apply (subgoal_tac "ASID s = ASID t" , simp)
+   apply blast
+  apply (cases s , cases t , clarsimp simp: state.defs)
+  done
+
+
+lemma mmu_translate_sat_abs_refine_pa'2:
+  "\<lbrakk> mmu_translate va s = (pa, s');  mmu_translate va t = (pa', t') ;
+           va \<notin> incon_set2 (tlb_incon_set'2 t) ; tlb_rel_abs'2 (typ_incon' s) (typ_incon'2 t) \<rbrakk> \<Longrightarrow> 
+                                          pa = pa'"
+  apply (frule_tac s = s in tlb_rel_abs_consistent'2 , simp)
+  apply (frule tlb_rel'_absD2 , clarsimp)
+  apply (clarsimp simp: mmu_translate_tlb_incon_state'_ext_def  mmu_translate_tlb_incon_state'2_ext_def Let_def split_def)
+  by (clarsimp simp: raise'exception_def split:if_split_asm)
+  
+lemma mmu_translate_abs_rel'2:
+  "\<lbrakk>  mmu_translate va t = (pa', t')\<rbrakk>  \<Longrightarrow> (t'::'a tlb_incon_state'2_scheme) = t\<lparr>exception := exception t'\<rparr>"
+  by (clarsimp simp: mmu_translate_tlb_incon_state'2_ext_def Let_def raise'exception_def split: if_split_asm)
+
+
+lemma mmu_translate_sat_abs_refine'2:
+   "\<lbrakk> mmu_translate va s = (pa, s');  mmu_translate va t = (pa', t') ;
+           va \<notin> incon_set2 (tlb_incon_set'2 t) ; tlb_rel_abs'2 (typ_incon' s) (typ_incon'2 t) \<rbrakk> \<Longrightarrow> 
+            tlb_rel_abs'2  (typ_incon' s') (typ_incon'2 t')"
+  apply (frule_tac s = s in tlb_rel_abs_consistent'2 ; clarsimp )
+  apply (frule tlb_rel'_absD2 , clarsimp)
+  apply (clarsimp simp: tlb_rel_abs'2_def)
+  apply (subgoal_tac "s' = s\<lparr>exception := exception s'\<rparr> \<and> t' = t\<lparr>exception := exception t'\<rparr>")
+   apply (subgoal_tac "exception t' = exception s'")
+    apply (cases t, cases t, cases s, cases s', clarsimp simp: state.defs saturated_no_flt_def)
+   prefer 2
+   apply (frule mmu_translate_abs_rel', clarsimp)
+   apply (frule mmu_translate_abs_rel'2, clarsimp)
+  apply (clarsimp simp: mmu_translate_tlb_incon_state'_ext_def mmu_translate_tlb_incon_state'2_ext_def Let_def)
+  apply (subgoal_tac "(ASID s, va) \<notin> incon_set (tlb_incon_set' s)")
+   apply (clarsimp simp: Let_def raise'exception_def split: if_split_asm)
+  by force
+
+
+lemma mmu_translate_sat_abs_refine_consistency2:
+   "\<lbrakk> mmu_translate va s = (pa, s');  mmu_translate va t = (pa', t') ;
+           va \<notin> incon_set2 (tlb_incon_set'2 t) ; tlb_rel_abs'2 (typ_incon' s) (typ_incon'2 t) \<rbrakk> \<Longrightarrow> 
+                                  va \<notin> incon_set2 (tlb_incon_set'2 t')"
+  apply (frule tlb_rel'_absD2 , clarsimp)
+  apply (clarsimp simp: mmu_translate_tlb_incon_state'_ext_def mmu_translate_tlb_incon_state'2_ext_def Let_def)
+  apply (subgoal_tac "(ASID s, va) \<notin> incon_set (tlb_incon_set' s)")
+   apply (clarsimp simp: Let_def raise'exception_def split: if_split_asm)
+  by force
+
+lemma mmu_translate_sat_no_flt_abs_refine2:
+  "\<lbrakk> mmu_translate va s = (pa, s');  mmu_translate va t = (pa', t') ;
+           va \<notin> incon_set2 (tlb_incon_set'2 t) ; tlb_rel_abs'2 (typ_incon' s) (typ_incon'2 t) \<rbrakk> \<Longrightarrow> 
+                              pa = pa' \<and>  tlb_rel_abs'2  (typ_incon' s') (typ_incon'2 t')  \<and> 
+                              va \<notin> incon_set2 (tlb_incon_set'2 t')"
+  by (clarsimp simp: mmu_translate_sat_abs_refine_pa'2 mmu_translate_sat_abs_refine'2
+      mmu_translate_sat_abs_refine_consistency2)
+
 
 end
