MMU_ARMv7_Refinement_No_Fault/ARMv7_Mem_Write_Read_Ref.thy
@@ -164,6 +164,49 @@ definition
 end
 
 
+
+instantiation tlb_incon_state'2_ext :: (type) mem_op    
+begin
+
+definition   
+  "(mmu_read  :: (vaddr  \<Rightarrow>  'a tlb_incon_state'2_scheme \<Rightarrow> bool list \<times>  'a tlb_incon_state'2_scheme))
+   \<equiv>  \<lambda>va. do {
+                     pa  \<leftarrow> mmu_translate va;
+                     mem1 pa
+  }"
+
+definition
+ "(mmu_read_size  :: (vaddr \<times> nat \<Rightarrow>  'a tlb_incon_state'2_scheme \<Rightarrow> bool list \<times>  'a tlb_incon_state'2_scheme))
+  \<equiv> \<lambda>(va,size). do {
+                     pa  \<leftarrow> mmu_translate va;
+                     mem_read1 (pa , size)
+  }"
+
+
+definition   
+  "(mmu_write_size  :: (bool list \<times> vaddr \<times> nat \<Rightarrow> 'a tlb_incon_state'2_scheme \<Rightarrow> unit \<times> 'a tlb_incon_state'2_scheme))
+  \<equiv> \<lambda>(value, vaddr, size). do {
+      ttbr0 <- read_state TTBR0;
+      asid  <- read_state ASID;
+      mem   <- read_state MEM; 
+      paddr <- mmu_translate vaddr;
+      tlb_incon_set <- read_state tlb_incon_set'2; 
+      exception <- read_state exception;
+      if exception = NoException 
+        then  do {
+                   write'mem1 (value, paddr, size);
+                   mem' <- read_state MEM;
+                   let ptable_asid_va = ptable_comp asid mem mem' ttbr0 ttbr0;
+                   let incon_set_n = incon_set2 tlb_incon_set \<union> snd ` ptable_asid_va;
+                   let tlb_incon_set = tlb_incon_set \<lparr>incon_set2 := incon_set_n \<rparr>;
+                   update_state (\<lambda>s. s\<lparr> tlb_incon_set'2 :=  tlb_incon_set \<rparr>)
+            }
+        else return ()
+   }"
+  instance ..
+end
+
+
 lemma mem1_exception:
   "mem1 p b = (val, r) \<Longrightarrow>  r = b\<lparr>exception := exception r\<rparr>"
   apply (clarsimp simp: mem1_def)
@@ -2086,6 +2129,70 @@ lemma write_refinement_saturated_incon_only:
    apply (simp add: write'mem1_eq_ASID_TTBR0)
    done
 
+lemma mmu_incon_eq_ASID_TTBR0_MEM:
+  "\<lbrakk> mmu_translate va (s::'a tlb_incon_state'_scheme) = (pa , s') \<rbrakk>  \<Longrightarrow> ASID s = ASID s' \<and> TTBR0 s = TTBR0 s' \<and>
+                     MEM s = MEM s'"
+  apply (clarsimp simp: mmu_translate_tlb_incon_state'_ext_def Let_def)
+  by (clarsimp simp:raise'exception_def Let_def split: if_split_asm)+
+
+
+lemma  to_do:
+  "{v. (ASID b, v) \<in> ptable_comp (ASID b) (MEM b) (MEM bc) (TTBR0 b) (TTBR0 b)}
+           \<subseteq> snd ` ptable_comp (ASID b) (MEM b) (MEM bc) (TTBR0 b) (TTBR0 b)"
+  apply (clarsimp simp: subset_image_iff)
+  apply (rule_tac x = "ptable_comp (ASID b) (MEM b) (MEM bc) (TTBR0 b) (TTBR0 b)" in exI)
+  apply (rule conjI)
+   apply simp
+  apply (clarsimp simp: ptable_comp_def)
+  apply (clarsimp simp: snd_eq_Range)
+  by auto
+  
+
+lemma write_refinement_incon_incon_only2:        
+  "\<lbrakk> mmu_write_size (val,va, sz) s = ((), s');  va \<notin> incon_set2 (tlb_incon_set'2 t);
+          tlb_rel_abs'2 (typ_incon' s) (typ_incon'2 t) ;  mmu_write_size (val,va, sz) t = ((), t')  \<rbrakk> \<Longrightarrow> 
+                                 tlb_rel_abs'2 (typ_incon' s') (typ_incon'2 t')"  
+  apply (frule_tac s = s in tlb_rel_abs_consistent'2 ; clarsimp )
+  apply (frule_tac tlb_rel'_absD2 , clarsimp)
+  apply (clarsimp simp: mmu_write_size_tlb_incon_state'2_ext_def  mmu_write_size_tlb_incon_state'_ext_def)
+  apply (cases "mmu_translate va s" ,cases "mmu_translate va t" , clarsimp)
+  apply (frule_tac t=t and pa'= aa and t' = ba in   mmu_translate_sat_no_flt_abs_refine2)  apply clarsimp+
+  apply (clarsimp simp: tlb_rel_abs'2_def)
+  apply (subgoal_tac "exception b = exception ba")
+   prefer 2 apply (case_tac b , case_tac ba , clarsimp simp: state.defs)
+  apply (clarsimp split: if_split_asm)
+  apply (case_tac "write'mem1 (val, aa, sz) b " , case_tac "write'mem1 (val, aa, sz) ba" , clarsimp simp: Let_def)
+  apply (subgoal_tac "state.truncate bb = state.truncate bc")
+   prefer 2 
+  using write_mem_state_trun_equal apply blast
+  apply (rule conjI , clarsimp simp: state.defs)
+  apply (subgoal_tac "MEM bb = MEM bc  \<and> MEM s = MEM b" , simp)
+   apply (subgoal_tac "ASID s = ASID b \<and> TTBR0 s = TTBR0 b" , simp)
+
+    prefer 2
+  using mmu_incon_eq_ASID_TTBR0_MEM apply blast
+   prefer 2
+   apply (rule conjI)
+    apply (clarsimp simp: state.defs)
+  using mmu_incon_eq_ASID_TTBR0_MEM
+   apply blast
+  apply (rule conjI)
+   apply clarsimp
+   apply (subgoal_tac "ASID bb = ASID b" , simp)
+  using write'mem1_eq_ASID_TTBR0 apply blast
+  apply (subgoal_tac "ASID bb = ASID b" , simp)
+
+   apply (subgoal_tac 
+      "{v. (ASID b, v) \<in> incon_set (tlb_incon_set' b) }
+           \<subseteq> incon_set2 (tlb_incon_set'2 ba)")
+    apply (subgoal_tac "{v.  (ASID b, v) \<in> ptable_comp (ASID b) (MEM b) (MEM bc) (TTBR0 b) (TTBR0 b)}
+           \<subseteq> snd ` ptable_comp (ASID b) (MEM b) (MEM bc) (TTBR0 b) (TTBR0 b)")
+     apply blast
+    prefer 2
+    apply clarsimp
+   apply (clarsimp simp: to_do)
+  using write'mem1_eq_ASID_TTBR0 apply blast
+  done
 
 
 (* refinement for read theroems *)
@@ -2218,6 +2325,45 @@ lemma  mem_read1_consistent_tlb_rel_abs:
      apply (clarsimp simp: mem1_def raise'exception_def split: option.splits if_split_asm)
     apply (clarsimp simp: raise'exception_def split: option.splits if_split_asm)
    apply (clarsimp simp: tlb_rel_abs'_def state.defs)
+  done
+
+
+
+lemma  mem_read1_consistent_tlb_rel_abs2:
+  "\<lbrakk>mem_read1 (a, sz) s = (val, s'); mem_read1 (a, sz) t = (val, t'); 
+             va \<notin> incon_set2 (tlb_incon_set'2 t); tlb_rel_abs'2 (typ_incon' s) (typ_incon'2 t)\<rbrakk>
+              \<Longrightarrow>  va \<notin> incon_set2 (tlb_incon_set'2 t') \<and>  tlb_rel_abs'2 (typ_incon' s') (typ_incon'2 t')"
+  apply (rule conjI)
+   apply (subgoal_tac "ASID t = ASID t' \<and> incon_set2 (tlb_incon_set'2 t) = incon_set2 (tlb_incon_set'2 t')")
+    apply clarsimp
+   apply (drule mem1_read_exception)
+   apply (drule mem1_read_exception)
+   apply (cases t, cases t')
+   apply clarsimp
+  apply (subgoal_tac "exception s' =  exception t'")
+   apply (drule mem1_read_exception)
+   apply (drule mem1_read_exception)
+   apply (clarsimp simp: tlb_rel_abs'2_def)
+   apply (rule conjI)
+    apply (clarsimp simp: state.defs)
+    apply (cases s', cases t')
+    apply clarsimp
+   apply (rule conjI)
+    apply (cases s', cases t')
+    apply clarsimp
+    apply (subgoal_tac "ASID t = ASID t' \<and> incon_set2 (tlb_incon_set'2 t) = incon_set2 (tlb_incon_set'2 t')")
+    apply clarsimp
+   apply (cases t, cases t')
+   apply clarsimp
+   apply (subgoal_tac "MEM s = MEM t \<and> exception s = exception t")
+    apply (clarsimp simp: mem_read1_def)
+    apply (clarsimp split: if_split_asm)
+        apply (clarsimp simp: mem1_def raise'exception_def split: option.splits if_split_asm)
+       apply (clarsimp simp: mem1_def raise'exception_def split: option.splits if_split_asm)
+      apply (clarsimp simp: mem1_def raise'exception_def split: option.splits if_split_asm)
+     apply (clarsimp simp: mem1_def raise'exception_def split: option.splits if_split_asm)
+    apply (clarsimp simp: raise'exception_def split: option.splits if_split_asm)
+   apply (clarsimp simp: tlb_rel_abs'2_def state.defs)
   done
 
 
